src/SLImp/Util.v
@@ -1,0 +1,63 @@
+Lemma not_None_iff_Some : forall n (m : nat),
+   (n = Some m <-> n <> None).
+Proof.
+Admitted.
+
+Program Definition hassn_sub (X: id) a (Q : Assertion) : Assertion :=
+  mk_asn (fun h st => forall n, (find (aeval st a) h) = Some n -> Q h (ImpDependencies.update st X n)) _.
+Next Obligation.
+  unfold read.
+(**
+  unfold ImpDependencies.update, read.
+  rewrite <- H.
+ *) 
+Admitted.
+
+Lemma in_update_extend : forall (st : state) (h : Heap) (e : aexp) (e' : nat) (X : id),
+  In (aeval st e) h -> 
+  aeval st e = aeval (ImpDependencies.update st X e') e ->
+  In (aeval (ImpDependencies.update st X e') e) h.
+Proof.
+  intros.
+  rewrite <- H0.
+  assumption.
+Qed.
+
+Lemma aeval_update_extend : forall (st : state) (e : aexp) (e' : nat) (X : id),
+  aeval st e = aeval (ImpDependencies.update st X e') e.
+Proof.
+  intros.
+  induction e.
+  simpl. reflexivity.
+  simpl. rewrite update_neq. reflexivity.
+  
+Admitted.
+
+Fixpoint free_in_heap_prop (a n : nat) (h : Heap) : Prop :=
+  match n with
+  | 0    => True
+  | S n' => not (In a h) /\ free_in_heap_prop (a+1) (n') h
+  end.
+  
+Program Definition free a n : Assertion :=
+  mk_asn (fun h st => free_in_heap_prop (aeval st a) n h) _.
+Next Obligation.
+Admitted.
+
+(**
+Theorem hoare_allocate : forall X n a Q,
+  {{ free a n //\\ ((a |-> (ANum 0)) -* assn_sub X a Q) }} X &= ALLOC n {{ Q }}.
+Proof.
+  intros X n a Q st st' Hc Pre.
+  inversion Hc. subst. simpl in *.
+  inversion Pre.
+  apply H0.
+  
+  split.
+    inversion Hc. subst.
+    simpl in *.
+*)    
+
+(** 
+{{ empSP }} X &= ALLOC n {{ aexp_eq (AId X) a //\\ ((ANum a) |-> (ANum 0)) ** (((APlus (ANum a) (ANum 1)) |-> ANum 0)) }}.
+*)
